\begin{figure}[H]
\centering
\begin{subequations}
	\begin{equation}
		\Delta = N \sum{x^2} - {\biggl(\sum{x}\biggr)}^2,
	\end{equation}
	\begin{equation}
		a_{\text{Reg}} = \frac{N\sum{x\cdot y} - \sum{x} \cdot \sum{y}}{\Delta},
	\end{equation}
    \begin{equation}
		b_{\text{Reg}} = \frac{\sum{x^2} \cdot \sum{y} - \sum{x} \cdot \sum{x \cdot y}}{\Delta},
	\end{equation}
	\begin{equation}
		\sigma_{y} = \sqrt{\frac{\sum{(y - a_{\text{Reg}} \cdot x - b_{\text{Reg}})^2}}{N - 2}},
	\end{equation}
	\begin{equation}
		\sigma_{a} = \sigma_{y} \sqrt{\frac{N}{\Delta}},
	\end{equation}
	\begin{equation}
		\sigma_{b} = \sigma_{y} \sqrt{\frac{\sum{x^2}}{\Delta}}
	\end{equation}

	\label{eq:regress}
\end{subequations}
\end{figure}